Split invertibility into two files.

core/properties/invertibility/left_invertibility.v
@@ -10,23 +10,16 @@ From core.modeling
 From core.properties.injectivity 
   Require Import Injectivity.
 
-From core.properties.surjectivity 
-  Require Import surjectivity.
 
 
 (*************************************************************)
-(** * Surjectivity of CoqTL (Model)                          *)
+(** * Left invertibility in CoqTL                            *)
 (** * Using operational semantics                            *)
 (*************************************************************)
 
 Definition Left_Invertible {tc:TransformationConfiguration} (tr:Transformation) :=
     exists (tr_inv: Transformation (tc:= InverseTC tc)), forall (sm:SourceModel) (tm:TargetModel),
       (execute tr sm) = tm -> (execute tr_inv tm) = sm.
-
-
-Definition Right_Invertible {tc:TransformationConfiguration} (tr:Transformation) :=
-    exists (tr_inv: Transformation (tc:= InverseTC tc)), forall (sm:SourceModel) (tm:TargetModel),
-      (execute tr_inv tm) = sm -> (execute tr sm) = tm.
 
 
 Lemma left_invertible_injective {tc:TransformationConfiguration} : 
@@ -55,24 +48,4 @@ Proof.
 Qed.
 
 
-Lemma right_invertible_surjective {tc:TransformationConfiguration} : 
-  forall tr, Right_Invertible tr -> Surjectivity tr.
-Proof.
- intro tr.
- unfold Right_Invertible.
- intros (tr_inv & H).
- unfold Surjectivity.
- intro tm.
- exists (execute tr_inv tm).
- apply H.
- reflexivity. 
-Qed.
-
-
-Corollary not_surjective_not_invertible :
-   forall (tc:TransformationConfiguration) tr, 
-      (~ Surjectivity tr) -> ~ Right_Invertible tr.
-Proof.
-  intros tc tr H ; contradict H ; apply right_invertible_surjective ; assumption.
-Qed.
 
