core/properties/invertibility/right_invertibility.v
@@ -1,0 +1,45 @@
+From Stdlib 
+  Require Import String EqNat List PeanoNat Lia FunctionalExtensionality.
+
+From core 
+  Require Import Semantics Syntax Model TransformationConfiguration Certification utils.Utils.
+
+From core.modeling 
+  Require Import ConcreteSyntax ModelingSemantics ModelingMetamodel ConcreteExpressions Parser.
+
+
+From core.properties.surjectivity 
+  Require Import surjectivity.
+
+
+(*************************************************************)
+(** * Right invertibility in CoqTL                           *)
+(** * Using operational semantics                            *)
+(*************************************************************)
+
+Definition Right_Invertible {tc:TransformationConfiguration} (tr:Transformation) :=
+    exists (tr_inv: Transformation (tc:= InverseTC tc)), forall (sm:SourceModel) (tm:TargetModel),
+      (execute tr_inv tm) = sm -> (execute tr sm) = tm.
+
+
+Lemma right_invertible_surjective {tc:TransformationConfiguration} : 
+  forall tr, Right_Invertible tr -> Surjectivity tr.
+Proof.
+ intro tr.
+ unfold Right_Invertible.
+ intros (tr_inv & H).
+ unfold Surjectivity.
+ intro tm.
+ exists (execute tr_inv tm).
+ apply H.
+ reflexivity. 
+Qed.
+
+
+Corollary not_surjective_not_invertible :
+   forall (tc:TransformationConfiguration) tr, 
+      (~ Surjectivity tr) -> ~ Right_Invertible tr.
+Proof.
+  intros tc tr H ; contradict H ; apply right_invertible_surjective ; assumption.
+Qed.
+
